moving things out of the poorly named examples/unit-tests directory; turned the --pretype flag on by default

lib/prims.fst
@@ -15,112 +15,435 @@
 *)
 module Prims
 
-type l_and : E => E => P
-type l_or  : E => E => P
-type l_not : E => P
-type l_iff : E => E => P
-type l_implies : E => E => P
-type Forall : 'a:S => ('a => E) => E
-type Exists : 'a:S => ('a => E) => E
-type Relational : E => E
-type DoubleSided : E => E
-type SPEC_ONLY : E => E
-type True : P
-type False : P
-type EqTyp : E => E => E
-type Eq : 'a:S => 'a => 'a => P
-type Eq2 : 'a:S => 'b:S => 'a => 'b => P
-type TypeOf : 'a:S => 'a => E
-logic tfun type AsE : 'a:S => 'a => E
-type neq2 : _ = fun ('a:S) ('b:S) (x:'a) (y:'b) => x<>y
-type neq : _ = fun ('a:S) (x:'a) (y:'a) => x<>y
-type KindOf : E => E
-type Not : _ = fun ('P:E) => (l_not 'P)
-type XOR : _ = fun ('P:E) ('Q:E) => (l_and (l_or 'P 'Q) (Not(l_and 'P 'Q)))
-type ITE : _ = fun ('P:E) ('Q:E) ('R:E) => ('P ==> 'Q) /\ ((l_not 'P) ==> 'R)
-type object
+kind Unop  = Type => Type           (* simple kind abbreviation *)
+kind Binop = Type => Type => Type   
+type l_not : Unop  (* prefix unary '~' *)
+type l_and : Binop (* infix binary '/\' *)
+type l_or  : Binop (* infix binary '\/' *)
+type l_iff : Binop (* infix binary '<==>' *)
+type l_imp : Binop (* infix binary '==>' *)
+type Forall : #'a:Type => ('a => Type) => Type 
+type Exists : #'a:Type => ('a => Type) => Type 
+type ForallTyp : (Type => Type) => Type (* Handled specially by the type-checker to support quantification over types of arbitrary kinds *)
+type ExistsTyp : (Type => Type) => Type (* Handled specially by the type-checker to support quantification over types of arbitrary kinds *)
+type True : Type
+type False : Type
+type EqTyp : Type => Type => Type                    (* infix binary '==' *)
+type Eq2 : #'a:Type => #'b:Type => 'a => 'b => Type  (* infix binary '==' *)
+type TypeOf : #'a:Type => 'a => Type
+type KindOf : Type => Type
+type XOR ('P:Type) ('Q:Type) = ('P \/ 'Q) /\ ~('P /\ 'Q)
+type ITE ('P:Type) ('Q:Type) ('R:Type) = ('P ==> 'Q) /\ (~'P ==> 'R) (* if/then/else in concrete syntax at the level of types/formulae *)
+
+monad_lattice { (* The definition of the PURE effect is fixed; no user should ever change this *)
+  PURE::
+             terminating
+             kind Pre = Type
+             kind Post ('a:Type) = 'a => Type
+             kind WP ('a:Type) = Post 'a => Pre
+             type return   ('a:Type) (x:'a) ('p:Post 'a) = 'p x
+             type bind_wp  ('a:Type) ('b:Type) ('wp1:WP 'a) ('wlp1:WP 'a) ('wp2: 'a => WP 'b) ('wlp2:'a => WP 'b) ('p:Post 'b) = 'wp1 (fun a => 'wp2 a 'p)
+             type bind_wlp ('a:Type) ('b:Type) ('wlp1:WP 'a) ('wlp2:'a => WP 'b) ('p:Post 'b) = 'wlp1 (fun a => 'wlp2 a 'p)
+             type ite_wlp ('a:Type) ('wlp_cases:WP 'a) ('post:Post 'a) =
+                 (forall (a:'a). 'post a \/ 'wlp_cases (fun a1 => a=!=a1))
+             type ite_wp ('a:Type) ('wlp_cases:WP 'a) ('wp_cases:WP 'a) ('post:Post 'a) =
+                 (forall (a:'a). 'post a \/ 'wlp_cases (fun a' => a=!=a'))
+                 /\ ('wp_cases (fun a => True))
+             type wp_binop ('a:Type) ('wp1:WP 'a) ('op:Type => Type => Type) ('wp2:WP 'a) ('p:Post 'a) =
+                 'op ('wp1 'p) ('wp2 'p)
+             type wp_as_type ('a:Type) ('wp:WP 'a) = (forall ('p:Post 'a). 'wp 'p)
+             type close_wp ('a:Type) ('b:Type) ('wp:'b => WP 'a) ('p:Post 'a) = (forall (b:'b). 'wp b 'p)
+             type close_wp_t ('a:Type) ('wp:Type => WP 'a) ('p:Post 'a) = (forall ('b:Type). 'wp 'b 'p)
+             type assert_p ('a:Type) ('P:Type) ('wp:WP 'a) ('p:Post 'a) = ('P /\ ('P ==> 'wp 'p))
+             type assume_p ('a:Type) ('P:Type) ('wp:WP 'a) ('p:Post 'a) = ('P ==> 'wp 'p)
+             with Pure ('a:Type) ('pre:Pre) ('post:Post 'a) =
+                 PURE 'a
+                   (fun ('p:Post 'a) => 'pre /\ (forall a. 'pre /\ 'post a ==> 'p a)) (* WP *)
+                   (fun ('p:Post 'a) => forall a. 'pre /\ 'post a ==> 'p a)           (* WLP *)
+             and Tot ('a:Type) =
+                 PURE 'a (fun 'p => (forall (x:'a). 'p x)) (fun 'p => (forall (x:'a). 'p x))
+}
+type assert_pure ('a:Type) ('P:Type) : PURE.WP 'a = fun ('post:PURE.Post 'a) => 'P /\ ('P ==> (forall (x:'a). 'post x))
+type assume_pure ('a:Type) ('P:Type) : PURE.WP 'a = fun ('post:PURE.Post 'a) => 'P ==> (forall (x:'a). 'post x)
+
 type bool
+type b2t (b:bool) = b==true
 type unit
-assume Unit_id: forall (x:unit). x=()
+assume Unit_id: forall (x:unit). x==()
 type int
 type char
 type byte
-type int32
+type uint16
+type int32 = int
 type int64
-type double
+type float
+type double = float
 type string
-type ref : S => S
-type LBL : string => E => E
+type array : Type => Type
+type ref : Type => Type
+type LBL : string => Type => Type
 type bytes
+type exn
 
-logic data type Tuple2: 'a:S 
-          => 'b:('a => S)
-          => S = 
-  | MkTuple2: 'a:S 
-           -> 'b:('a => S) 
-           -> fst:'a 
-           -> snd:'b fst 
+logic data type option 'a =
+  | None : option 'a
+  | Some : v:'a -> option 'a
+
+type heap
+logic val SelHeap : #'a:Type -> heap -> ref 'a -> 'a
+logic val UpdHeap : #'a:Type -> heap -> ref 'a -> 'a -> heap
+logic val EmpHeap : heap
+logic val InHeap  : #'a:Type -> heap -> ref 'a -> bool
+assume SelUpd1: forall ('a:Type) (h:heap) (x:ref 'a) (v:'a).{:pattern (SelHeap (UpdHeap h x v) x)} SelHeap (UpdHeap h x v) x == x
+assume SelUpd2: forall ('a:Type) ('b:Type) (h:heap) (x:ref 'a) (y:ref 'b) (v:'b).{:pattern (SelHeap (UpdHeap h y v) x)} y=!=x ==> SelHeap (UpdHeap h y v) x == SelHeap h x
+assume InHeap1:  forall ('a:Type) (h:heap) (x:ref 'a) (v:'a).{:pattern (InHeap (UpdHeap h x v) x)} InHeap (UpdHeap h x v) x == true
+assume InHeap2:  forall ('a:Type) ('b:Type) (h:heap) (x:ref 'a) (y:ref 'b) (v:'b).{:pattern (InHeap (UpdHeap h y v) x)} y=!=x ==> InHeap (UpdHeap h y v) x == InHeap h x
+
+type refset
+logic val EmptySet : refset
+logic val Singleton : ref 'a -> refset
+logic val Union : refset -> refset -> refset
+logic val Intersection : refset -> refset -> refset
+type InSet : #'a:Type => ref 'a => refset => Type
+type SetEqual : refset => refset => Type
+assume InEmptySet:     forall a. ~(InSet a EmptySet)
+assume InSingleton:    forall a. InSet a (Singleton a)
+assume InSingletonInv: forall a b. InSet a (Singleton b) <==> a==b
+assume InUnion:        forall s1 s2 a. InSet a (Union s1 s2) <==> (InSet a s1 \/ InSet a s1)
+assume InUnionL:       forall s1 s2 a. InSet a s1 ==> InSet a (Union s1 s2)
+assume InUnionR:       forall s1 s2 a. InSet a s2 ==> InSet a (Union s1 s2)
+assume UnionIdemL:     forall s1 s2. Union (Union s1 s2) s2 == Union s1 s2
+assume UnionIdemR:     forall s1 s2. Union s1 (Union s1 s2) == Union s1 s2
+assume InInter:        forall s1 s2 a. InSet a (Intersection s1 s2) <==> (InSet a s1 /\ InSet a s2)
+assume InterIdemL:     forall s1 s2. Intersection (Intersection s1 s2) s2 == Intersection s1 s2
+assume InterdemR:      forall s1 s2. Intersection s1 (Intersection s1 s2) == Intersection s1 s2
+assume SetEqualDef:    forall s1 s2. SetEqual s1 s2 <==> (forall a. InSet a s1 <==> InSet a s2)
+assume SeqEqualExt:    forall s1 s2. SetEqual s1 s2 ==> s1==s2
+logic data type refs =
+  | AllRefs : refs
+  | SomeRefs : v:refset -> refs
+
+(* let zoo = function  *)
+(*   | AllRefs -> AllRefs *)
+(*   | SomeRefs v -> SomeRefs v *)
+assume val modifies : r:refs -> PURE.Tot (x:refs{x==r})
+(* let modifies (r:refs) = r *)
+(* let f1 x = *)
+(*   let r = modifies x in *)
+(*   AllRefs *)
+
+(* let foo (b:bool) = if b then 0 else 1 *)
+(* let bar a b = a *)
+
+type Modifies (mods:refs) (h:heap) (h':heap) =
+    (if b2t (is_AllRefs mods)
+     then True
+     else forall 'b (x:ref 'b). (b2t (InHeap h x) /\ ~(InSet x (SomeRefs.v mods))) ==> (b2t (InHeap h' x) /\ SelHeap h x==SelHeap h' x))
+
+logic data type result : Type => Type =
+  | V : 'a:Type -> v:'a -> result 'a
+  | E : 'a:Type -> e:exn -> result 'a
+  | Err : 'a:Type -> msg:string -> result 'a
+
+assume val retype : result 'a -> PURE.Tot (result 'b)
+(* let retype r = match r with *)
+(*   | V _ -> Err "impos" *)
+(*   | Err m -> Err m *)
+(*   | E e -> E e *)
+
+monad_lattice {
+  STATE::
+             kind Pre     = heap => Type
+             kind Post ('a:Type) = 'a => heap => Type
+             kind WP ('a:Type) = Post 'a => Pre
+             type return   ('a:Type) (x:'a) ('p:Post 'a) = 'p x
+             type bind_wp  ('a:Type) ('b:Type) ('wp1:WP 'a) ('wlp1:WP 'a) ('wp2:'a => WP 'b) ('wlp2:'a => WP 'b) ('p:Post 'b) (h0:heap) = 'wp1 (fun a => 'wp2 a 'p) h0
+             type bind_wlp ('a:Type) ('b:Type) ('wlp1:WP 'a) ('wlp2:'a => WP 'b) ('p:Post 'b) (h0:heap) = 'wlp1 (fun a => 'wlp2 a 'p) h0
+             type ite_wlp  ('a:Type) ('wlp_cases:WP 'a) ('post:Post 'a) (h0:heap) =
+                 (forall (a:'a) (h:heap). 'post a h \/ 'wlp_cases (fun a1 h1 => a=!=a1 /\ h=!=h1) h0)
+             type ite_wp ('a:Type) ('wlp_cases:WP 'a) ('wp_cases:WP 'a) ('post:Post 'a) (h0:heap) =
+                 (forall (a:'a) (h:heap). 'post a h \/ 'wlp_cases (fun a1 h1 => a=!=a1 /\ h=!=h1) h0)
+                 /\ 'wp_cases (fun a h_ => True) h0
+             type wp_binop ('a:Type) ('wp1:WP 'a) ('op:Type => Type => Type) ('wp2:WP 'a) ('p:Post 'a) (h:heap) =
+                 'op ('wp1 'p h) ('wp2 'p h)
+             type wp_as_type ('a:Type) ('wp:WP 'a) = (forall ('p:Post 'a) (h:heap). 'wp 'p h)
+             type close_wp ('a:Type) ('b:Type) ('wp:'b => WP 'a) ('p:Post 'a) (h:heap) = (forall (b:'b). 'wp b 'p h)
+             type close_wp_t ('a:Type) ('wp:Type => WP 'a) ('p:Post 'a) (h:heap) = (forall ('b:Type). 'wp 'b 'p h)
+             type assert_p ('a:Type) ('P:Type) ('wp:WP 'a) ('p:Post 'a) (h:heap) = ('P /\ ('P ==> 'wp 'p h))
+             type assume_p ('a:Type) ('P:Type) ('wp:WP 'a) ('p:Post 'a) (h:heap) = ('P ==> 'wp 'p h)
+             with ST ('a:Type) ('pre:Pre) ('post: heap => Post 'a) (mods:refs) =
+                 STATE 'a
+                   (fun ('p:Post 'a) (h:heap) => 'pre h /\ (forall a h1. ('pre h /\ Modifies mods h h1 /\ 'post h a h1) ==> 'p a h1)) (* WP *)
+                   (fun ('p:Post 'a) (h:heap) => (forall a h1. ('pre h /\ Modifies mods h h1 /\ 'post h a h1) ==> 'p a h1))           (* WLP *)
+;
+  EXN::
+             kind Pre  = Type
+             kind Post ('a:Type) = result 'a => Type
+             kind WP   ('a:Type) = Post 'a => Pre
+             type return ('a:Type) (x:'a) ('p:Post 'a) = 'p (V x)
+             type bind_wp ('a:Type) ('b:Type) ('wp1:WP 'a) ('wlp1:WP 'a) ('wp2:'a => WP 'b) ('wlp2:'a => WP 'b) ('p:Post 'b) =
+                 (forall (rb:result 'b). 'p rb \/ 'wlp1 (fun ra1 => if b2t (is_V ra1)
+                                                                    then 'wlp2 (V.v ra1) (fun rb2 => rb2=!=rb)
+                                                                    else ra1 =!= rb))
+                 /\ 'wp1 (fun ra1 => (ITE (b2t (is_V ra1))
+                                          ('wp2 (V.v ra1) (fun rb2 => True))
+                                           True))
+             type bind_wlp ('a:Type) ('b:Type) ('wlp1:WP 'a) ('wlp2:'a => WP 'b) ('p:Post 'b) =
+                 (forall (rb:result 'b). 'p rb \/ 'wlp1 (fun ra1 => if b2t (is_V ra1)
+                                                                    then 'wlp2 (V.v ra1) (fun rb2 => rb2=!=rb)
+                                                                    else  ra1 =!= rb))
+             type ite_wlp  ('a:Type) ('wlp_cases:WP 'a) ('post:Post 'a) =
+                 (forall (a:result 'a). 'post a \/ 'wlp_cases (fun a1 => a=!=a1))
+             type ite_wp ('a:Type) ('wlp_cases:WP 'a) ('wp_cases:WP 'a) ('post:Post 'a) =
+                 (forall (a:result 'a). 'post a \/ 'wlp_cases (fun a1 => a=!=a1))
+                 /\ 'wp_cases (fun ra2 => True)
+             type wp_binop ('a:Type) ('wp1:WP 'a) ('op:Type => Type => Type) ('wp2:WP 'a) ('p:Post 'a) =
+                 'op ('wp1 'p) ('wp2 'p)
+             type wp_as_type ('a:Type) ('wp:WP 'a) = (forall ('p:Post 'a). 'wp 'p)
+             type close_wp ('a:Type) ('b:Type) ('wp:'b => WP 'a) ('p:Post 'a) = (forall (b:'b). 'wp b 'p)
+             type close_wp_t ('a:Type) ('wp:Type => WP 'a) ('p:Post 'a)  = (forall ('b:Type). 'wp 'b 'p)
+             type assert_p ('a:Type) ('P:Type) ('wp:WP 'a) ('p:Post 'a) = ('P /\ ('P ==> 'wp 'p))
+             type assume_p ('a:Type) ('P:Type) ('wp:WP 'a) ('p:Post 'a) = ('P ==> 'wp 'p)
+             with Exn ('a:Type) ('pre:Pre) ('post:Post 'a) =
+                 EXN 'a
+                   (fun 'p => 'pre /\ (forall (r:result 'a). ('pre /\ 'post r) ==> 'p r)) (* WP *)
+                   (fun 'p => (forall (r:result 'a). ('pre /\ 'post r) ==> 'p r))         (* WLP *)
+ ;
+  ALL::
+             kind Pre  = heap => Type
+             kind Post ('a:Type) = result 'a => heap => Type
+             kind WP ('a:Type) = Post 'a => Pre
+             type return ('a:Type) (x:'a) ('p:Post 'a) = 'p (V x)
+             type bind_wp ('a:Type) ('b:Type) ('wp1:WP 'a) ('wlp1:WP 'a) ('wp2:'a => WP 'b) ('wlp2:'a => WP 'b) ('p:Post 'b) (h0:heap) =
+                 (forall rb h. 'p rb h \/ 'wlp1 (fun ra h1 => if b2t (is_V ra)
+                                                              then 'wlp2 (V.v ra) (fun rb2 h2 => ~(rb==rb2 \/ h==h2)) h1
+                                                              else ~(rb==ra \/ h==h1)) h0)
+                 /\ 'wp1 (fun ra h1 => if b2t (is_V ra)
+                                       then 'wp2 (V.v ra) (fun _a _b => True) h1
+                                       else True) h0
+             type bind_wlp ('a:Type) ('b:Type) ('wlp1:WP 'a) ('wlp2:'a => WP 'b) ('p:Post 'b) (h0:heap) =
+                 (forall rb h. 'p rb h \/ 'wlp1 (fun ra h1 => if b2t (is_V ra)
+                                                              then 'wlp2 (V.v ra) (fun rb2 h2 => ~(rb==rb2 \/ h==h2)) h1
+                                                              else ~(rb==ra \/ h==h1)) h0)
+             type ite_wlp  ('a:Type) ('wlp_cases:WP 'a) ('post:Post 'a) (h0:heap) =
+                 (forall (ra:result 'a) (h:heap). 'post ra h \/ 'wlp_cases (fun ra2 h2 => ra=!=ra2 /\ h=!=h2) h0)
+             type ite_wp ('a:Type) ('wlp_cases:WP 'a) ('wp_cases:WP 'a) ('post:Post 'a) (h0:heap) =
+                 (forall (ra:result 'a) (h:heap). 'post ra h \/ 'wlp_cases (fun ra2 h2 => ra=!=ra2 /\ h=!=h2) h0)
+                 /\ 'wp_cases (fun _a _b => True) h0
+             type wp_binop ('a:Type) ('wp1:WP 'a) ('op:Type => Type => Type) ('wp2:WP 'a) ('p:Post 'a) (h:heap) =
+                 'op ('wp1 'p h) ('wp2 'p h)
+             type wp_as_type ('a:Type) ('wp:WP 'a) = (forall ('p:Post 'a) (h:heap). 'wp 'p h)
+             type close_wp ('a:Type) ('b:Type) ('wp:'b => WP 'a) ('p:Post 'a) (h:heap) = (forall (b:'b). 'wp b 'p h)
+             type close_wp_t ('a:Type) ('wp:Type => WP 'a) ('p:Post 'a) (h:heap) = (forall ('b:Type). 'wp 'b 'p h)
+             type assert_p ('a:Type) ('P:Type) ('wp:WP 'a) ('p:Post 'a) (h:heap) = ('P /\ ('P ==> 'wp 'p h))
+             type assume_p ('a:Type) ('P:Type) ('wp:WP 'a) ('p:Post 'a) (h:heap) = ('P ==> 'wp 'p h)
+             with All ('a:Type) ('pre:Pre) ('post: heap => Post 'a) (mods:refs) =
+                 ALL 'a
+                   (fun ('p:Post 'a) (h:heap) => 'pre h /\ (forall ra h1. ('pre h /\ Modifies mods h h1 /\ 'post h ra h1) ==> 'p ra h1)) (* WP *)
+                   (fun ('p:Post 'a) (h:heap) => forall ra h1. ('pre h /\ Modifies mods h h1 /\ 'post h ra h1) ==> 'p ra h1)             (* WLP *)
+             and ML ('a:Type) =
+                 ALL 'a (fun ('p:Post 'a) (h0:heap) => forall (a:result 'a) (h:heap). 'p a h)
+                        (fun ('p:Post 'a) (h0:heap) => forall (a:result 'a) (h:heap). 'p a h)
+
+  with
+  PURE  ~> STATE = (fun ('a:Type) ('wp:PURE.WP 'a) ('p:STATE.Post 'a) (h:heap) => 'wp (fun a => 'p a h));
+  STATE ~> ALL   = (fun ('a:Type) ('wp:STATE.WP 'a) ('p:ALL.Post 'a) => 'wp (fun a => 'p (V a)));
+  PURE  ~> EXN   = (fun ('a:Type) ('wp:PURE.WP 'a) ('p:EXN.Post 'a) => 'wp (fun a => 'p (V a)));
+  EXN   ~> ALL   = (fun ('a:Type) ('wp:EXN.WP 'a) ('p:ALL.Post 'a) (h:heap) => 'wp (fun ra => 'p ra h))
+}
+
+type Tuple2 'a 'b =
+  | MkTuple2: _1:'a
+           -> _2:'b
            -> Tuple2 'a 'b
 
-logic data type Tuple3: 'a:S 
-          => 'b:('a => S) 
-          => 'c:(x:'a => 'b x => S) 
-          => S = 
-  | MkTuple3: 'a:S 
-           -> 'b:('a => S) 
-           -> 'c:(x:'a => 'b x => S)
-           -> fst:'a 
-           -> snd:'b fst 
-           -> _3:'c fst snd 
+type Tuple3 'a 'b 'c =
+  | MkTuple3: _1:'a
+           -> _2:'b
+           -> _3:'c
            -> Tuple3 'a 'b 'c
 
-logic data type Tuple4: 'a:S 
-          => 'b:(x:'a => S)
-          => 'c:(x:'a => 'b x => S) 
-          => 'd:(x:'a => y:'b x => z:'c x y => S) 
-          => S = 
-  | MkTuple4: 'a:S 
-           -> 'b:('a => S) 
-           -> 'c:(x:'a => 'b x => S)
-           -> 'd:(x:'a => y:'b x => z:'c x y => S) 
-           -> fst:'a 
-           -> snd:'b fst 
-           -> _3:'c fst snd 
-           -> _4:'d fst snd _3
+type Tuple4 'a 'b 'c 'd =
+  | MkTuple4: _1:'a
+           -> _2:'b
+           -> _3:'c
+           -> _4:'d
            -> Tuple4 'a 'b 'c 'd
 
-logic data type Tuple5: 'a:S 
-          => 'b:('a => S)
-          => 'c:(x:'a => 'b x => S) 
-          => 'd:(x:'a => y:'b x => z:'c x y => S) 
-          => 'e:(x:'a => y:'b x => z:'c x y => w:'d x y z => S) 
-          => S = 
-  | MkTuple5: 'a:S 
-           -> 'b:('a => S) 
-           -> 'c:(x:'a => 'b x => S)
-           -> 'd:(x:'a => y:'b x => z:'c x y => S) 
-           -> 'e:(x:'a => y:'b x => z:'c x y => w:'d x y z => S) 
-           -> fst:'a 
-           -> snd:'b fst 
-           -> _3:'c fst snd 
-           -> _4:'d fst snd _3
-           -> _5:'e fst snd _3 _4
-           -> Tuple4 'a 'b 'c 'd 'e
+type Tuple5 'a 'b 'c 'd 'e =
+  | MkTuple5: _1:'a
+           -> _2:'b
+           -> _3:'c
+           -> _4:'d
+           -> _5:'e
+           -> Tuple5 'a 'b 'c 'd 'e
 
-type exn
-type float
-type result : S => S =
-  | V : 'a:S -> v:'a -> result 'a
-  | E : 'a:S -> e:exn -> result 'a
-  | Err : 'a:S -> result 'a
-logic val L : 'a -> 'a
-logic val R : 'a -> 'a
+type Tuple6 'a 'b 'c 'd 'e 'f =
+  | MkTuple6: _1:'a
+           -> _2:'b
+           -> _3:'c
+           -> _4:'d
+           -> _5:'e
+           -> _6:'f
+           -> Tuple6 'a 'b 'c 'd 'e 'f
+
+
+type Tuple7 'a 'b 'c 'd 'e 'f 'g =
+  | MkTuple7: _1:'a
+           -> _2:'b
+           -> _3:'c
+           -> _4:'d
+           -> _5:'e
+           -> _6:'f
+           -> _7:'g
+           -> Tuple7 'a 'b 'c 'd 'e 'f 'g
+
+
+type Tuple8 'a 'b 'c 'd 'e 'f 'g 'h =
+  | MkTuple8: _1:'a
+           -> _2:'b
+           -> _3:'c
+           -> _4:'d
+           -> _5:'e
+           -> _6:'f
+           -> _7:'g
+           -> _8:'h
+           -> Tuple8 'a 'b 'c 'd 'e 'f 'g 'h
+
+type DTuple2: 'a:Type
+          => 'b:('a => Type)
+          => Type =
+  | MkDTuple2: 'a:Type
+           -> 'b:('a => Type)
+           -> _1:'a
+           -> _2:'b _1
+           -> DTuple2 'a 'b
+
+type DTuple3: 'a:Type
+          => 'b:('a => Type)
+          => 'c:(x:'a => 'b x => Type)
+          => Type =
+  | MkDTuple3: 'a:Type
+           -> 'b:('a => Type)
+           -> 'c:(x:'a => 'b x => Type)
+           -> _1:'a
+           -> _2:'b _1
+           -> _3:'c _1 _2
+           -> DTuple3 'a 'b 'c
+
+type DTuple4: 'a:Type
+          => 'b:(x:'a => Type)
+          => 'c:(x:'a => 'b x => Type)
+          => 'd:(x:'a => y:'b x => z:'c x y => Type)
+          => Type =
+  | MkDTuple4: 'a:Type
+           -> 'b:('a => Type)
+           -> 'c:(x:'a => 'b x => Type)
+           -> 'd:(x:'a => y:'b x => z:'c x y => Type)
+           -> _1:'a
+           -> _2:'b _1
+           -> _3:'c _1 _2
+           -> _4:'d _1 _2 _3
+           -> DTuple4 'a 'b 'c 'd
+
+(* logic data type Tuple5: 'a:Type *)
+(*           => 'b:('a => Type) *)
+(*           => 'c:(x:'a => 'b x => Type) *)
+(*           => 'd:(x:'a => y:'b x => z:'c x y => Type) *)
+(*           => 'e:(x:'a => y:'b x => z:'c x y => w:'d x y z => Type) *)
+(*           => Type = *)
+(*   | MkTuple5: 'a:Type *)
+(*            -> 'b:('a => Type) *)
+(*            -> 'c:(x:'a => 'b x => Type) *)
+(*            -> 'd:(x:'a => y:'b x => z:'c x y => Type) *)
+(*            -> 'e:(x:'a => y:'b x => z:'c x y => w:'d x y z => Type) *)
+(*            -> _1:'a *)
+(*            -> _2:'b _1 *)
+(*            -> _3:'c _1 _2 *)
+(*            -> _4:'d _1 _2 _3 *)
+(*            -> _5:'e _1 _2 _3 _4 *)
+(*            -> Tuple5 'a 'b 'c 'd 'e *)
+
+(* logic data type Tuple6: 'a:Type *)
+(*           => 'b:('a => Type) *)
+(*           => 'c:(x:'a => 'b x => Type) *)
+(*           => 'd:(x:'a => y:'b x => z:'c x y => Type) *)
+(*           => 'e:(x:'a => y:'b x => z:'c x y => w:'d x y z => Type) *)
+(*           => 'f:(x:'a => y:'b x => z:'c x y => w:'d x y z => u:'e x y z w => Type) *)
+(*           => Type = *)
+(*   | MkTuple6: 'a:Type *)
+(*            -> 'b:('a => Type) *)
+(*            -> 'c:(x:'a => 'b x => Type) *)
+(*            -> 'd:(x:'a => y:'b x => z:'c x y => Type) *)
+(*            -> 'e:(x:'a => y:'b x => z:'c x y => w:'d x y z => Type) *)
+(*            -> 'f:(x:'a => y:'b x => z:'c x y => w:'d x y z => v:'e x y z w => Type) *)
+(*            -> _1:'a *)
+(*            -> _2:'b _1 *)
+(*            -> _3:'c _1 _2 *)
+(*            -> _4:'d _1 _2 _3 *)
+(*            -> _5:'e _1 _2 _3 _4 *)
+(*            -> _6:'f _1 _2 _3 _4 _5 *)
+(*            -> Tuple6 'a 'b 'c 'd 'e 'f *)
+
+(* logic data type Tuple7: 'a:Type *)
+(*           => 'b:('a => Type) *)
+(*           => 'c:(x:'a => 'b x => Type) *)
+(*           => 'd:(x:'a => y:'b x => z:'c x y => Type) *)
+(*           => 'e:(x:'a => y:'b x => z:'c x y => w:'d x y z => Type) *)
+(*           => 'f:(x:'a => y:'b x => z:'c x y => w:'d x y z => u:'e x y z w => Type) *)
+(*           => 'g:(x:'a => y:'b x => z:'c x y => w:'d x y z => u:'e x y z w => v:'f x y z w u => Type) *)
+(*           => Type = *)
+(*   | MkTuple7: 'a:Type *)
+(*            -> 'b:('a => Type) *)
+(*            -> 'c:(x:'a => 'b x => Type) *)
+(*            -> 'd:(x:'a => y:'b x => z:'c x y => Type) *)
+(*            -> 'e:(x:'a => y:'b x => z:'c x y => w:'d x y z => Type) *)
+(*            -> 'f:(x:'a => y:'b x => z:'c x y => w:'d x y z => u:'e x y z w => Type) *)
+(*            -> 'g:(x:'a => y:'b x => z:'c x y => w:'d x y z => u:'e x y z w => v:'f x y z w u => Type) *)
+(*            -> _1:'a *)
+(*            -> _2:'b _1 *)
+(*            -> _3:'c _1 _2 *)
+(*            -> _4:'d _1 _2 _3 *)
+(*            -> _5:'e _1 _2 _3 _4 *)
+(*            -> _6:'f _1 _2 _3 _4 _5 *)
+(*            -> _7:'g _1 _2 _3 _4 _5 _6 *)
+(*            -> Tuple7 'a 'b 'c 'd 'e 'f 'g *)
+
+(* logic data type Tuple8: 'a:Type *)
+(*           => 'b:('a => Type) *)
+(*           => 'c:(a:'a => 'b a => Type) *)
+(*           => 'd:(a:'a => b:'b a => c:'c a b => Type) *)
+(*           => 'e:(a:'a => b:'b a => c:'c a b => d:'d a b c => Type) *)
+(*           => 'f:(a:'a => b:'b a => c:'c a b => d:'d a b c => e:'e a b c d => Type) *)
+(*           => 'g:(a:'a => b:'b a => c:'c a b => d:'d a b c => e:'e a b c d => f:'f a b c d e => Type) *)
+(*           => 'h:(a:'a => b:'b a => c:'c a b => d:'d a b c => e:'e a b c d => f:'f a b c d e => g:'g a b c d e f => Type) *)
+(*           => Type = *)
+(*   | MkTuple8: 'a:Type *)
+(*            -> 'b:('a => Type) *)
+(*            -> 'c:(a:'a => 'b a => Type) *)
+(*            -> 'd:(a:'a => b:'b a => c:'c a b => Type) *)
+(*            -> 'e:(a:'a => b:'b a => c:'c a b => d:'d a b c => Type) *)
+(*            -> 'f:(a:'a => b:'b a => c:'c a b => d:'d a b c => e:'e a b c d => Type) *)
+(*            -> 'g:(a:'a => b:'b a => c:'c a b => d:'d a b c => e:'e a b c d => f:'f a b c d e => Type) *)
+(*            -> 'h:(a:'a => b:'b a => c:'c a b => d:'d a b c => e:'e a b c d => f:'f a b c d e => g:'g a b c d e f => Type) *)
+(*            -> _1:'a *)
+(*            -> _2:'b _1 *)
+(*            -> _3:'c _1 _2 *)
+(*            -> _4:'d _1 _2 _3 *)
+(*            -> _5:'e _1 _2 _3 _4 *)
+(*            -> _6:'f _1 _2 _3 _4 _5 *)
+(*            -> _7:'g _1 _2 _3 _4 _5 _6 *)
+(*            -> _8:'h _1 _2 _3 _4 _5 _6 _7 *)
+(*            -> Tuple8 'a 'b 'c 'd 'e 'f 'g 'h *)
 
 (* Primitive (structural) equality.
    What about for function types? *)
-val op_Equality : 'a:S -> 'b:S -> x:'a -> y:'b -> z:bool {(z=true <==> x=y) /\ (z=false <==> (x<>y))}
-type IfThenElse : 'P:E => (u:unit{'P} => E) => (u:unit{not 'P} => E) => E
-(* Integer arithmetic *)
+assume val op_Equality : 'a:Type -> 'b:Type -> 'a -> 'b -> PURE.Tot bool
+assume val op_disEquality : 'a:Type -> 'b:Type -> 'a -> 'b -> PURE.Tot bool
+(* assume val op_Equality : 'a:Type -> 'b:Type -> x:'a -> y:'b -> z:bool {(z==true <==> x==y) /\ (z==false <==> (x=!=y))} *)
+(* assume val op_disEquality : 'a:Type -> 'b:Type -> x:'a -> y:'b -> z:bool {(z==true <==> x=!=y) /\ (z==false <==> (x==y))} *)
+logic type IfThenElse : 'P:Type => (u:unit{'P} => Type) => (u:unit{~'P} => Type) => Type
+
 logic val Add : int -> int -> int
 logic val Sub : int -> int -> int
 logic val Mul : int -> int -> int
@@ -128,48 +451,72 @@ logic val Div : int -> int -> int
 logic val Minus : int -> int
 logic val Modulo : int -> int -> int
 
-type LT : int => int => E
-type GT : int => int => E
-type LTE : int => int => E
-type GTE : int => int => E
+type LT : int => int => Type
+type GT : int => int => Type
+type LTE : int => int => Type
+type GTE : int => int => Type
 type nat = i:int{i >= 0}
 type pos = n:nat{n > 0}
 
-logic data type option 'a =
-  | None : option 'a
-  | Some : v:'a -> option 'a
 
-type either 'a 'b =
+logic data type either 'a 'b =
   | Inl : v:'a -> either 'a 'b
   | Inr : v:'b -> either 'a 'b
 
-logic data type list 'a =
-  | Nil : list 'a
-  | Cons : hd:'a -> tl:list 'a -> list 'a
+logic data type list 'cc =
+  | Nil : list 'cc
+  | Cons : hd:'cc -> tl:list 'cc -> list 'cc
 
-val Assume: 'P:E -> unit -> (y:unit{'P})
-val Assert : 'P:E -> x:unit{'P} -> y:unit{'P}
-val lemma : 'P:E -> x:unit{'P} -> z:unit{'P}
-val unreachable : x:unit{LBL "unreachable" False} -> 'a
+assume val fst : ('a * 'b) -> PURE.Tot 'a
+assume val snd : ('a * 'b) -> PURE.Tot 'b
+assume val Assume: 'P:Type -> unit -> (y:unit{'P})
+assume val Assert : 'P:Type -> x:unit{'P} -> y:unit{'P}
+assume val lemma : 'P:Type -> x:unit{'P} -> z:unit{'P}
+assume val unreachable : x:unit{LBL "unreachable" False} -> 'a
+assume val failwith: string -> 'a (* TODO: refine with a monadic type *)
+assume val raise: exn -> 'a (* TODO: refine with a monadic type *)
+assume val pipe_right: 'a -> ('a -> 'b) -> 'b
+assume val pipe_left: ('a -> 'b) -> 'a -> 'b
+assume val ignore: 'a -> unit
+assume val exit: int -> 'a
+assume val try_with: (unit -> 'a) -> (exn -> 'a) -> 'a
 
-(* Primitive functions with trusted specs  *)
-val _dummy_op_ColonEquals: ref 'a -> 'a -> unit
-val _dummy_op_Dereference: ref 'a -> 'a
-val _dummy_op_AmpAmp             : x:bool -> y:bool -> z:bool { z=true ==>  x=true /\  y=true}
-val _dummy_op_BarBar             : x:bool -> y:bool -> z:bool { (z=true ==> x=true \/  y=true) /\
-                                                                (z=false ==> x=false /\ y=false) }
-val _dummy_op_Negation           : x:bool -> y:bool { (y=true ==> x=false) /\ (y=false ==> x=true) }
+(* Unrefined specifications for these functions for typing ML code *)
+assume val op_ColonEquals: ref 'a -> 'a -> unit
+assume val op_Dereference: ref 'a -> 'a
+assume val op_AmpAmp             : bool -> bool -> PURE.Tot bool
+assume val op_BarBar             : bool -> bool -> PURE.Tot bool
+assume val op_Negation           : bool -> PURE.Tot bool
+assume val op_Multiply           : int -> int -> PURE.Tot int
+assume val op_Division           : int -> int -> int
+assume val op_Subtraction        : int -> int -> PURE.Tot int
+assume val op_Addition           : int -> int -> PURE.Tot int
+assume val op_Minus              : int -> PURE.Tot int
+assume val op_Modulus            : int -> int -> int
+assume val op_LessThanOrEqual    : int -> int -> PURE.Tot bool
+assume val op_GreaterThan        : int -> int -> PURE.Tot bool
+assume val op_GreaterThanOrEqual : int -> int -> PURE.Tot bool
+(* TODO: < in operators clashes with t<..> notation. Fix *)
+assume val op_LessThan           : int -> int -> PURE.Tot bool
 
-val _dummy_op_Multiply           : x:int -> y:int -> z:int{z=x*y}
-val _dummy_op_Division           : x:int -> y:int{y<>0} -> z:int{z=x/y}
-val _dummy_op_Subtraction        : x:int -> y:int -> z:int{z=x-y}
-val _dummy_op_Addition           : x:int -> y:int -> z:int{z=x+y}
-val _dummy_op_Minus              : x:int -> y:int{y=Minus x}
-val _dummy_op_Modulus            : x:int -> y:int -> z:int{z=x%y}
+(* (\* (\\* Primitive functions with trusted specs  *\\) *\) *)
+(* (\* assume val op_ColonEquals: ref 'a -> 'a -> unit *\) *)
+(* (\* assume val op_Dereference: ref 'a -> 'a *\) *)
+(* (\* assume val op_AmpAmp             : x:bool -> y:bool -> z:bool { z==true ==>  x==true /\  y==true} *\) *)
+(* (\* assume val op_BarBar             : x:bool -> y:bool -> z:bool { (z==true ==> x==true \/  y==true) /\ *\) *)
+(* (\*                                                                 (z==false ==> x==false /\ y==false) } *\) *)
+(* (\* assume val op_Negation           : x:bool -> y:bool { (y==true ==> x==false) /\ (y==false ==> x==true) } *\) *)
 
-val _dummy_op_LessThanOrEqual : x:int -> y:int -> z:bool{(z=true ==> x <= y) /\ (z=false ==> x > y)}
-val _dummy_op_GreaterThan : x:int -> y:int -> z:bool{(z=true ==> x > y) /\ (z=false ==> x <= y)}
+(* (\* assume val op_Multiply           : x:int -> y:int -> z:int{z==x*y} *\) *)
+(* (\* assume val op_Division           : x:int -> y:int{y=!=0} -> z:int{z==x/y} *\) *)
+(* (\* assume val op_Subtraction        : x:int -> y:int -> z:int{z==x-y} *\) *)
+(* (\* assume val op_Addition           : x:int -> y:int -> z:int{z==x+y} *\) *)
+(* (\* assume val op_Minus              : x:int -> y:int{y==Minus x} *\) *)
+(* (\* assume val op_Modulus            : x:int -> y:int -> z:int{z==x%y} *\) *)
+(* (\* assume val op_LessThanOrEqual : x:int -> y:int -> z:bool{(z==true ==> x <= y) /\ (z==false ==> x > y)} *\) *)
+(* (\* assume val op_GreaterThan : x:int -> y:int -> z:bool{(z==true ==> x > y) /\ (z==false ==> x <= y)} *\) *)
 
-(* TODO: >= in operators clashes with t<..> notation. Fix *)
-(* val _dummy_op_GreaterThanOrEqual : x:int -> y:int -> z:bool{(z=true ==> x >= y) /\ (z=false ==> x < y) } *)
-(* val _dummy_op_LessThan : x:int -> y:int -> z:bool{(z=true ==> x < y) /\ (z=false ==> x >= y)} *)
+(* (\* (\\* TODO: < in operators clashes with t<..> notation. Fix *\\) *\) *)
+(* (\* assume val op_GreaterThanOrEqual : x:int -> y:int -> bool(\\* {(z=true ==> x >= y) /\ (z=false ==> x < y) } *\\) *\) *)
+(* (\* assume val op_LessThan : x:int -> y:int -> bool(\\* {(z=true ==> x < y) /\ (z=false ==> x >= y)} *\\\) *\\) *\) *)
+    
