examples/unit-tests/ocaml-backend-stub.fst
@@ -1,10 +1,18 @@
+(*********************************************************************************)
 module FSharp.Format
 type doc 
 assume val pretty: int -> doc -> string
 
+(*********************************************************************************)
+module Microsoft.FStar.Backends.OCaml
+open Microsoft.FStar.Absyn.Syntax
+assume val pp_module: modul -> string
+
+(*********************************************************************************)
 module Microsoft.FStar.Backends.OCaml.Syntax
 type mllib
 
+(*********************************************************************************)
 module Microsoft.FStar.Backends.OCaml.ASTTrans
 open Microsoft.FStar
 open Microsoft.FStar.Absyn.Syntax
@@ -14,7 +22,9 @@ assume val string_of_error : error -> string
 exception OCamlFailure of Range.range * error
 assume val mlmod_of_fstars : list<modul> -> mllib
 
+(*********************************************************************************)
 module Microsoft.FStar.Backends.OCaml.Code
 open Microsoft.FStar.Backends.OCaml.Syntax
-
 assume val doc_of_mllib: mllib -> FSharp.Format.doc
+(*********************************************************************************)
+
